- Create a truth table for

  $\neg$(p$\lor$q) ^ ($\neg$ p$\land$ $\neg$q)

  |  P   |  q   | $\neg$p | $\neg$q | (p$\lor$q) | $\neg$(p$\lor$q) | ($\neg$p  $\land \neg$ q) | $\neg$(p$\lor$q) $\land$ ($\neg$p$\land \neg$q) |
  | :--: | :--: | :-----: | :-----: | :--------: | :--------------: | :-----------------------: | :--------------------------------------: |
  |  T   |  T   |    F    |    F    |     T      |        F         |             F             |                    F                     |
  |  T   |  F   |    F    |    T    |     T      |        F         |             F             |                    F                     |
  |  F   |  T   |    T    |    F    |     T      |        F         |             F             |                    F                     |
  |  F   |  F   |    T    |    T    |     F      |        T         |             T             |                    T                     |

- De Morgan's Law

  $\neg(p \lor q) = \neg p \land \neg q $

## $\iff$ Biconditional

- a $\iff$ b translation

- a if and only if b

- notation: iff = if and only if

- Two directions

  1. a => b (If a then b) (A implies B)
  2. a <= b (If b then a) (B implies A)
  3. or b => a

  - **You have to prove both directions, break it up into two pieces**

- $\neg p  \land (p \lor \neg q)$

- p = I will study 5 hours per day

- q = I will get an A in discrete math

  - (Sidenote) $A\land (B \lor C) = (A \land B) \lor (A\land C)$


  - |  A   |  B   |  C   | $(B\lor C)$ | $A \land (B \lor C)$ | $(A\land B)$ | $(A\land C)$ | $(A\land B) \lor (A\land C)$ |
    | :--: | :--: | :--: | :---------: | :------------------: | :----------: | :----------: | :--------------------------: |
    |  T   |  T   |  T   |      T      |          T           |      T       |      T       |              T               |
    |  T   |  T   |  F   |      T      |          T           |      T       |      F       |              T               |
    |  T   |  F   |  T   |      T      |          T           |      F       |      T       |              T               |
    |  T   |  F   |  F   |      F      |          F           |      F       |      F       |              F               |
    |  F   |  T   |  T   |      T      |          F           |      F       |      F       |              F               |
    |  F   |  T   |  F   |      T      |          F           |      F       |      F       |              F               |
    |  F   |  F   |  T   |      T      |          F           |      F       |      F       |              F               |
    |  F   |  F   |  F   |      F      |          F           |      F       |      F       |              F               |



Prove or disprove the following claim.

$n^2 + 1$ is odd if and only if n is even

###Steps

1. Identify p and q

   - p = $n^2+1$ is odd

   - q = n is even

   - $p \iff q$

   - Evens are of the form 2K

     Odds are of the form 2K+1

I. If p then q

If $n^2+1$ is odd then n is even

Proof: The above is impossible to prove, so we can do $\neg q \rightarrow \neg p$

The <u>way</u> to prove this is to use the contrapositive. Recall that p &rarr; q is equivalent to $\neg q \rightarrow \neg p$

If n is odd then $n^2 + 1$ is even

Proof: If n is odd then n = 2k + 1 and $n^2 + 1$ = $(2K + 1)^2 + 1$

​									   = $4k^2 + 4k + 2$

​									   = $2(2k^2+2k+1) = even$



II. If q then p

If n is even then $n^2+1$ is odd

Proof: If n is even then n = 2K, and $n^2 + 1$ = $4K^2+1$

​									 = $2(2K^2) + 1$

​									 = even + 1

​									 = odd